Public service

hulls.v
@@ -105,7 +105,7 @@ Definition step145 csq_orig :=
   let csq_new := TS.fold (step1 csq_orig) csq_orig TS.empty in
   let csq_new' := TS.fold (step4 csq_orig) csq_orig csq_new in
   let csq_new'' := TS.fold (step5 csq_orig) csq_orig csq_new' in
-  if TS.is_empty csq_new then
+  if TS.is_empty csq_new'' then
     inl csq_orig
   else
     inr (TS.union csq_orig csq_new).
@@ -252,39 +252,25 @@ Proof.
   intros. apply step5_aux_correct; auto.
 Qed.
 
-Lemma conseq_congr: forall s1 s2 k (EQ: TS.Equal s1 s2),
-    Conseq s1 k -> Conseq s2 k.
-Proof.
-  intros. unfold TS.Equal in EQ. induction H; firstorder.
-  + constructor 3 with d; firstorder.
-  + constructor 4 with b d; firstorder.
-Qed.
-
-Lemma conseqs_congr: forall s1 s2 k (EQ: TS.Equal s1 s2),
-    Conseqs_imm s1 k -> Conseqs_imm s2 k.
-Proof.
-Admitted.
-(*
-  intros.
-  induction H.
-  + econstructor 1. eauto using conseq_congr.
-  + econstructor 2; eauto.
-Qed.
-*)
-
 Lemma fold_step_correct :
   forall csq_new csq_orig step,
     Conseqs_imm csq_orig csq_new ->
     step_correct step ->
     Conseqs_imm csq_orig (TS.fold (step csq_orig) csq_orig csq_new).
 Proof.
-  Hint Resolve conseq_congr conseqs_congr.
   intros; eapply SetProps.fold_rec_nodep; intros; eauto.
 Qed.
 
 Lemma step145_correct : forall ts, Conseqs_imm ts (csq_proj (step145 ts)).
 Proof.
+  Require Import DLib.
+  intros ts t H. destruct (step145 ts) eqn:eq. 
+  + simpl in *. unfold step145 in eq. flatten eq.
+    apply TS.is_empty_spec in Eq. apply SetProps.empty_is_empty_1 in Eq. eauto.
+  + simpl in *. unfold step145 in *. flatten eq.
+    constructor. 
 
+    
 Admitted.
 
 Inductive Conseqs : TS.t -> TS.t -> Prop :=
